cp

examples/wysteria/examples/fstar_main/traces.fst
@@ -407,7 +407,7 @@ let rec ith_row_from #a #b p i from =
 // 	    (decreases (stop_col - cur))
 // let rec lemma_ith_row #a #b p row stop_col cur w = 
 //   if index p row cur <> Equal then lemma_ith_row p row stop_col (cur + 1) w
-
+ 
 val row_as_list: sb:seq int -> r:seq entry{Seq.length r = Seq.length sb} -> i:bound sb -> Tot (list int)
   (decreases (Seq.length sb - i))
 let rec row_as_list sb r i = 
@@ -416,6 +416,12 @@ let rec row_as_list sb r i =
   else if Seq.index r i = Elim
   then row_as_list sb r (i + 1)
   else Seq.index sb i :: row_as_list sb r (i + 1)
+
+assume val row_as_list_eq: sb:seq int 
+		  -> r1:seq entry{Seq.length r1 = Seq.length sb}
+		  -> r2:seq entry{Seq.length r2 = Seq.length sb}
+		  -> i:bound sb{forall (x:ix sb). i <= x ==> Seq.index r1 x = Seq.index r2 x}
+		  -> Lemma (row_as_list sb r1 i = row_as_list sb r2 i)
  
 val iter_extends: a:_ -> b:_ 
 		-> i':bound a -> j':bound b
@@ -462,35 +468,35 @@ let next_row_wraparound a b i = iter_extends a b i (Seq.length b) (i + 1) 0
 // val lemma_next_row_eq: #a:seq int -> #b:seq int -> i:ix a{i+1 < Seq.length a} -> j:ix b -> x:ix b -> p:iter a b i j
 //   Lemma (ensures (index p 
 
-val lemma_next_row_unchanged: #a:seq int -> #b:seq int -> i:ix a{i+1 < Seq.length a} -> j:ix b -> k:bound b -> x:ix b{j < x}
+val lemma_next_row_unchanged: #a:seq int -> #b:seq int -> i:ix a{i+1 < Seq.length a} -> j:ix b -> k:bound b 
   -> p:iter a b i j
   -> q:iter a b i k
   -> Lemma (requires (index p i j = Unknown /\ j < k /\ Seq.index a i = Seq.index b j))
-	  (ensures ((index q (i + 1) x = index p i x) /\ index q (i + 1) j = Elim /\ index q i x = Elim))
+	  (ensures (forall (x:ix b{j < x}). (index q (i + 1) x = index p i x) 
+				       /\ index q (i + 1) j = Elim 
+				       /\ index q i x = Elim))
           (decreases k)
-let rec lemma_next_row_unchanged #a #b i j k x p q = 
+let rec lemma_next_row_unchanged #a #b i j k p q = 
   if j+1=k 
   then iter_extends a b i j i k
   else let q' = iter_i_j a b i (k - 1) in
-       let _ = lemma_next_row_unchanged #a #b i j (k - 1) x p q' in
+       let _ = lemma_next_row_unchanged #a #b i j (k - 1) p q' in
        iter_extends a b i (k - 1) i k
 
 val lemma_next_row_aux: #a:seq int -> #b:seq int -> i:ix a -> j:ix b  
       -> p:iter a b i j{index p i j = Unknown} 
       -> q:iter a b (i + 1) 0{Seq.index a i = Seq.index b j}
-      -> k:ix b{j < k}
       -> Lemma 
-  (requires True)
-  (ensures (index q i j = Equal 
+      (index q i j = Equal 
 	    /\ (i + 1 < Seq.length a 
  	       ==> (index q (i + 1) j = Elim
-  	           /\ index q (i + 1) k = index p i k))))
-let lemma_next_row_aux #a #b i j p q k = 
+  	           /\ (forall (k:ix b{j < k}). index q (i + 1) k = index p i k))))
+let lemma_next_row_aux #a #b i j p q = 
     iter_step a b i j (i + 1) 0 p q;
     next_row_wraparound #a #b i;
     if i + 1 < Seq.length a
-    then lemma_next_row_unchanged #a #b i j (Seq.length b) k p q
- 
+    then lemma_next_row_unchanged #a #b i j (Seq.length b) p q
+
 val lemma_next_row: #a:seq int -> #b:seq int -> i:ix a -> j:ix b  
       -> p:iter a b i j{index p i j = Unknown} 
       -> q:iter a b (i + 1) 0{Seq.index a i = Seq.index b j}
@@ -498,15 +504,14 @@ val lemma_next_row: #a:seq int -> #b:seq int -> i:ix a -> j:ix b
   (requires True)
   (ensures (index q i j = Equal 
 	    /\ (i + 1 < Seq.length a 
- 	       ==> (index q (i + 1) j = Elim
-  	           /\ row_as_list b (Matrix2.row q (i + 1)) j
-  	    	      = Cons.tl (row_as_list b (Matrix2.row p i) j)))))
+ 	       ==> (index q (i + 1) j = Elim 
+  	           /\ row_as_list b (row q (i + 1)) j
+  	    	      = Cons.tl (row_as_list b (row p i) j)))))
 let lemma_next_row #a #b i j p q = 
-    lemma_next_row_aux #a #b i j p q
-
-    iter_step a b i j (i + 1) 0 p q;
-    admit() //TODO: REMOVE ... boring
- 
+      lemma_next_row_aux #a #b i j p q; 
+      if (i + 1 < Seq.length a)
+      then row_as_list_eq b (row p i) (row q (i + 1)) (j + 1)
+  
 assume val advance:  a:Seq.seq int -> b:Seq.seq int -> i:ix a -> j:ix b
 	    -> p:iter a b i j
 	    -> q:iter a b (i + 1) 0
